Fixing the problem that some lambdas are not expanded away

books/projects/smtlink/verified/expand-cp.lisp
@@ -26,781 +26,823 @@
   :parents (verified)
   :short "Function expansion"
 
-(acl2::defevaluator-fast expev expev-lst
-                         ((if a b c) (equal a b) (not a)
-                          (cons a b) (binary-+ a b)
-                          (typespec-check ts x)
-                          (iff a b)
-                          (implies a b)
-                          (hint-please hint)
-                          (return-last x y z))
-                         :namedp t)
+  (acl2::defevaluator-fast expev expev-lst
+                           ((if a b c) (equal a b) (not a)
+                            (cons a b) (binary-+ a b)
+                            (typespec-check ts x)
+                            (iff a b)
+                            (implies a b)
+                            (hint-please hint)
+                            (return-last x y z))
+                           :namedp t)
 
-(acl2::def-ev-theoremp expev)
-(acl2::def-meta-extract expev expev-lst)
-(acl2::def-unify expev expev-alist)
+  (acl2::def-ev-theoremp expev)
+  (acl2::def-meta-extract expev expev-lst)
+  (acl2::def-unify expev expev-alist)
 
-(defalist sym-nat-alist
-  :key-type symbol
-  :val-type natp
-  :pred sym-nat-alistp
-  :true-listp t)
+  (defalist sym-nat-alist
+    :key-type symbol
+    :val-type natp
+    :pred sym-nat-alistp
+    :true-listp t)
 
-(local
- (defthm consp-of-sym-nat-alist-fix
-   (implies (consp (sym-nat-alist-fix x)) (consp x))
-   :hints (("Goal" :in-theory (enable sym-nat-alist-fix))))
- )
+  (local
+   (defthm consp-of-sym-nat-alist-fix
+     (implies (consp (sym-nat-alist-fix x)) (consp x))
+     :hints (("Goal" :in-theory (enable sym-nat-alist-fix))))
+   )
 
-(local
- (defthm len-of-sym-nat-alist-fix-<
-   (> (1+ (len x)) (len (sym-nat-alist-fix x)))
-   :hints (("Goal" :in-theory (enable sym-nat-alist-fix))))
- )
+  (local
+   (defthm len-of-sym-nat-alist-fix-<
+     (> (1+ (len x)) (len (sym-nat-alist-fix x)))
+     :hints (("Goal" :in-theory (enable sym-nat-alist-fix))))
+   )
 
-(local
- (defthm natp-of-cdar-sym-nat-alist-fix
-   (implies (consp (sym-nat-alist-fix x))
-            (natp (cdar (sym-nat-alist-fix x))))
-   :hints (("Goal" :in-theory (enable sym-nat-alist-fix))))
- )
+  (local
+   (defthm natp-of-cdar-sym-nat-alist-fix
+     (implies (consp (sym-nat-alist-fix x))
+              (natp (cdar (sym-nat-alist-fix x))))
+     :hints (("Goal" :in-theory (enable sym-nat-alist-fix))))
+   )
 
-(define update-fn-lvls ((fn symbolp) (fn-lvls sym-nat-alistp))
-  :returns (updated-fn-lvls sym-nat-alistp)
-  :measure (len fn-lvls)
-  :hints (("Goal" :in-theory (enable sym-nat-alist-fix)))
-  (b* ((fn (symbol-fix fn))
-       (fn-lvls (sym-nat-alist-fix fn-lvls))
-       ((unless (consp fn-lvls)) nil)
-       ((cons first rest) fn-lvls)
-       ((cons this-fn this-lvl) first)
-       ((unless (equal fn this-fn))
-        (cons (cons this-fn this-lvl)
-              (update-fn-lvls fn rest))))
-    (if (zp this-lvl)
-        (cons (cons this-fn 0) rest)
-      (cons (cons this-fn (1- this-lvl)) rest)))
-  ///
-  (more-returns
-   (updated-fn-lvls
-    (implies (and (symbolp fn)
-                  (sym-nat-alistp fn-lvls)
-                  (consp fn-lvls)
-                  (assoc-equal fn fn-lvls)
-                  (not (equal (cdr (assoc-equal fn fn-lvls)) 0)))
-             (< (cdr (assoc fn updated-fn-lvls))
-                (cdr (assoc fn fn-lvls))))
-    :name updated-fn-lvls-decrease))
-  )
-
-
-;; val-type can be a list of pseudo-termp
-;; This will give us two benefits: multiple facts and when it's nil,
-;; fact-finder fails to find a fact.
-(defalist fact-alist
-  :key-type pseudo-termp
-  :val-type pseudo-termp
-  :pred fact-alistp
-  :short "Value is the equivalence term about Key term."
-  :true-listp t)
-
-(defprod ex-args
-  :parents (function-expansion)
-  :short "Argument list for function expand"
-  ((fn-lvls sym-nat-alistp "Levels to expand each functions to."
-            :default nil)
-   (fn-lst func-alistp "List of function definitions to use for
-      function expansion." :default nil)
-   (facts fact-alistp "An alist of current learnt equivalence facts."
-          :default nil)
-   (fty-info fty-info-alist-p "FTY information." :default nil)
-   (wrld-fn-len natp "Number of function definitions in curent world."
-                :default 0)))
-
-(local
- (defthm natp-of-sum-lvls-lemma
-   (implies (and (consp (sym-nat-alist-fix fn-lvls)) (natp x))
-            (natp (+ (cdr (car (sym-nat-alist-fix fn-lvls))) x)))
-   :hints (("Goal"
-            :in-theory (enable sym-nat-alist-fix)
-            :use ((:instance natp-of-cdar-sym-nat-alist-fix)))))
- )
-
-(define sum-lvls ((fn-lvls sym-nat-alistp))
-  :returns (sum natp
-                :hints (("Goal"
-                         :use ((:instance natp-of-sum-lvls-lemma
-                                          (x (sum-lvls (cdr (sym-nat-alist-fix fn-lvls)))))))))
-  :measure (len fn-lvls)
-  :hints (("Goal" :in-theory (enable sym-nat-alist-fix)))
-  (b* ((fn-lvls (sym-nat-alist-fix fn-lvls))
-       ((unless (consp fn-lvls)) 0)
-       ((cons first rest) fn-lvls)
-       ((cons & lvl) first))
-    (+ lvl (sum-lvls rest)))
-  ///
-  (defthm sum-lvls-decrease-after-update
-    (implies (and (symbolp fn)
-                  (sym-nat-alistp fn-lvls)
-                  (consp fn-lvls)
-                  (assoc-equal fn fn-lvls)
-                  (not (equal (cdr (assoc-equal fn fn-lvls)) 0)))
-             (< (sum-lvls (update-fn-lvls fn fn-lvls))
-                (sum-lvls fn-lvls)))
-    :hints (("Goal" :in-theory (enable update-fn-lvls)))))
-
-(encapsulate ()
   (local (defthm alistp-of-pairlis$
            (alistp (acl2::pairlis$ a b))))
 
-  (local (defthm pseudo-term-substp-of-pairlis$-for-pseudo-lambda
-           (implies (and (pseudo-term-listp x) (pseudo-lambdap y))
-                    (acl2::pseudo-term-substp (pairlis$ (lambda-formals y) x)))))
+  (define update-fn-lvls ((fn symbolp) (fn-lvls sym-nat-alistp))
+    :returns (updated-fn-lvls sym-nat-alistp)
+    :measure (len fn-lvls)
+    :hints (("Goal" :in-theory (enable sym-nat-alist-fix)))
+    (b* ((fn (symbol-fix fn))
+         (fn-lvls (sym-nat-alist-fix fn-lvls))
+         ((unless (consp fn-lvls)) nil)
+         ((cons first rest) fn-lvls)
+         ((cons this-fn this-lvl) first)
+         ((unless (equal fn this-fn))
+          (cons (cons this-fn this-lvl)
+                (update-fn-lvls fn rest))))
+      (if (zp this-lvl)
+          (cons (cons this-fn 0) rest)
+        (cons (cons this-fn (1- this-lvl)) rest)))
+    ///
+    (more-returns
+     (updated-fn-lvls
+      (implies (and (symbolp fn)
+                    (sym-nat-alistp fn-lvls)
+                    (consp fn-lvls)
+                    (assoc-equal fn fn-lvls)
+                    (not (equal (cdr (assoc-equal fn fn-lvls)) 0)))
+               (< (cdr (assoc fn updated-fn-lvls))
+                  (cdr (assoc fn fn-lvls))))
+      :name updated-fn-lvls-decrease))
+    )
 
-  (define lambda-substitution ((fn-call pseudo-lambdap)
-                               (fn-actuals pseudo-term-listp))
-    :guard-hints (("Goal"
-                   :in-theory (e/d () (alistp-of-pairlis$
-                                       acl2::true-listp-when-symbol-listp))
-                   :use ((:instance acl2::true-listp-when-symbol-listp
-                                    (acl2::x (cadr fn-call)))
-                         (:instance alistp-of-pairlis$
-                                    (a (cadr fn-call))
-                                    (b fn-actuals)))))
+
+  ;; val-type can be a list of pseudo-termp
+  ;; This will give us two benefits: multiple facts and when it's nil,
+  ;; fact-finder fails to find a fact.
+  (defalist fact-alist
+    :key-type pseudo-termp
+    :val-type pseudo-termp
+    :pred fact-alistp
+    :short "Value is the equivalence term about Key term."
+    :true-listp t)
+
+  (defprod ex-args
+    :parents (function-expansion)
+    :short "Argument list for function expand"
+    ((fn-lvls sym-nat-alistp "Levels to expand each functions to."
+              :default nil)
+     (fn-lst func-alistp "List of function definitions to use for
+      function expansion." :default nil)
+     (facts fact-alistp "An alist of current learnt equivalence facts."
+            :default nil)
+     (fty-info fty-info-alist-p "FTY information." :default nil)
+     (wrld-fn-len natp "Number of function definitions in curent world."
+                  :default 0)))
+
+  (local
+   (defthm natp-of-sum-lvls-lemma
+     (implies (and (consp (sym-nat-alist-fix fn-lvls)) (natp x))
+              (natp (+ (cdr (car (sym-nat-alist-fix fn-lvls))) x)))
+     :hints (("Goal"
+              :in-theory (enable sym-nat-alist-fix)
+              :use ((:instance natp-of-cdar-sym-nat-alist-fix)))))
+   )
+
+  (define sum-lvls ((fn-lvls sym-nat-alistp))
+    :returns (sum natp
+                  :hints (("Goal"
+                           :use ((:instance natp-of-sum-lvls-lemma
+                                            (x (sum-lvls (cdr (sym-nat-alist-fix fn-lvls)))))))))
+    :measure (len fn-lvls)
+    :hints (("Goal" :in-theory (enable sym-nat-alist-fix)))
+    (b* ((fn-lvls (sym-nat-alist-fix fn-lvls))
+         ((unless (consp fn-lvls)) 0)
+         ((cons first rest) fn-lvls)
+         ((cons & lvl) first))
+      (+ lvl (sum-lvls rest)))
+    ///
+    (defthm sum-lvls-decrease-after-update
+      (implies (and (symbolp fn)
+                    (sym-nat-alistp fn-lvls)
+                    (consp fn-lvls)
+                    (assoc-equal fn fn-lvls)
+                    (not (equal (cdr (assoc-equal fn fn-lvls)) 0)))
+               (< (sum-lvls (update-fn-lvls fn fn-lvls))
+                  (sum-lvls fn-lvls)))
+      :hints (("Goal" :in-theory (enable update-fn-lvls)))))
+
+  (encapsulate ()
+
+    (local (defthm pseudo-term-substp-of-pairlis$-for-pseudo-lambda
+             (implies (and (pseudo-term-listp x) (pseudo-lambdap y))
+                      (acl2::pseudo-term-substp (pairlis$ (lambda-formals y) x)))))
+
+    (define lambda-substitution ((fn-call pseudo-lambdap)
+                                 (fn-actuals pseudo-term-listp))
+      :guard-hints (("Goal"
+                     :in-theory (e/d () (alistp-of-pairlis$
+                                         acl2::true-listp-when-symbol-listp))
+                     :use ((:instance acl2::true-listp-when-symbol-listp
+                                      (acl2::x (cadr fn-call)))
+                           (:instance alistp-of-pairlis$
+                                      (a (cadr fn-call))
+                                      (b fn-actuals)))))
+      :returns (subst-term
+                pseudo-termp
+                :hints (("Goal"
+                         :in-theory (e/d ()
+                                         (pseudo-term-substp-of-pairlis$-for-pseudo-lambda
+                                          acl2::return-type-of-substitute-into-term.xx))
+                         :use ((:instance
+                                pseudo-term-substp-of-pairlis$-for-pseudo-lambda
+                                (x fn-actuals)
+                                (y fn-call))
+                               (:instance
+                                acl2::return-type-of-substitute-into-term.xx
+                                (x (lambda-body (pseudo-lambda-fix fn-call)))
+                                (al (pairlis$ (lambda-formals
+                                               (pseudo-lambda-fix fn-call))
+                                              (pseudo-term-list-fix fn-actuals))))))))
+      (b* ((fn-call (pseudo-lambda-fix fn-call))
+           (fn-actuals (pseudo-term-list-fix fn-actuals))
+           (formals (lambda-formals fn-call))
+           (body (lambda-body fn-call)))
+        (acl2::substitute-into-term body (pairlis$ formals fn-actuals)))))
+
+  (local (defthm expev-alist-of-pairlis$
+           (equal (expev-alist (pairlis$ x y) a)
+                  (pairlis$ x (expev-lst y a)))))
+
+  (defthm lambda-substitution-correct
+    (implies (and (expev-meta-extract-global-facts)
+                  (alistp a)
+                  (pseudo-lambdap fn-call)
+                  (pseudo-term-listp fn-actuals))
+             (equal
+              (expev (lambda-substitution fn-call fn-actuals) a)
+              (expev (cons fn-call fn-actuals) a)))
+    :hints (("Goal"
+             :in-theory (enable lambda-substitution))))
+
+  (define function-substitution ((term pseudo-termp)
+                                 state)
     :returns (subst-term
               pseudo-termp
               :hints (("Goal"
                        :in-theory (e/d ()
-                                       (pseudo-term-substp-of-pairlis$-for-pseudo-lambda
-                                        acl2::return-type-of-substitute-into-term.xx))
+                                       (pseudo-termp
+                                        pseudo-term-listp
+                                        acl2::return-type-of-substitute-into-term.xx
+                                        acl2::return-type-of-simple-one-way-unify.a))
                        :use ((:instance
-                              pseudo-term-substp-of-pairlis$-for-pseudo-lambda
-                              (x fn-actuals)
-                              (y fn-call))
-                             (:instance
-                              acl2::return-type-of-substitute-into-term.xx
-                              (x (lambda-body (pseudo-lambda-fix fn-call)))
-                              (al (pairlis$ (lambda-formals
-                                             (pseudo-lambda-fix fn-call))
-                                            (pseudo-term-list-fix fn-actuals))))))))
-    (b* ((fn-call (pseudo-lambda-fix fn-call))
-         (fn-actuals (pseudo-term-list-fix fn-actuals))
-         (formals (lambda-formals fn-call))
-         (body (lambda-body fn-call)))
-      (acl2::substitute-into-term body (pairlis$ formals fn-actuals)))))
-
-(local (defthm expev-alist-of-pairlis$
-         (equal (expev-alist (pairlis$ x y) a)
-                (pairlis$ x (expev-lst y a)))))
-
-(defthm lambda-substitution-correct
-  (implies (and (expev-meta-extract-global-facts)
-                (alistp a)
-                (pseudo-lambdap fn-call)
-                (pseudo-term-listp fn-actuals))
-           (equal
-            (expev (lambda-substitution fn-call fn-actuals) a)
-            (expev (cons fn-call fn-actuals) a)))
-  :hints (("Goal"
-           :in-theory (enable lambda-substitution))))
-
-(define function-substitution ((term pseudo-termp)
-                               state)
-  :returns (subst-term
-            pseudo-termp
-            :hints (("Goal"
-                     :in-theory (e/d ()
-                                     (pseudo-termp
-                                      pseudo-term-listp
-                                      acl2::return-type-of-substitute-into-term.xx
-                                      acl2::return-type-of-simple-one-way-unify.a))
-                     :use ((:instance
-                            acl2::return-type-of-simple-one-way-unify.a
-                            (pat (cadr (acl2::meta-extract-formula-w
-                                        (symbol-fix fn-call)
-                                        (cdr (assoc-equal 'acl2::current-acl2-world
-                                                          (nth 2 state))))))
-                            (term (pseudo-term-fix term))
-                            (alist nil))))))
-  (b* ((term (pseudo-term-fix term))
-       ((unless (and (not (acl2::variablep term))
-                     (not (acl2::fquotep term))
-                     (symbolp (car term))))
-        (prog2$
-         (er hard? 'expand-cp=>function-substitution "expand-cp: fn-call is nil
+                              acl2::return-type-of-simple-one-way-unify.a
+                              (pat (cadr (acl2::meta-extract-formula-w
+                                          (symbol-fix fn-call)
+                                          (cdr (assoc-equal 'acl2::current-acl2-world
+                                                            (nth 2 state))))))
+                              (term (pseudo-term-fix term))
+                              (alist nil))))))
+    (b* ((term (pseudo-term-fix term))
+         ((unless (and (not (acl2::variablep term))
+                       (not (acl2::fquotep term))
+                       (symbolp (car term))))
+          (prog2$
+           (er hard? 'expand-cp=>function-substitution "expand-cp: fn-call is nil
                                or 'quote.")
-         nil))
-       ((cons fn-call &) term)
-       (formula (acl2::meta-extract-formula-w fn-call (w state)))
-       ((unless (pseudo-termp formula))
-        (prog2$
-         (er hard? 'expand-cp=>function-substitution "expand-cp: formula got by
+           nil))
+         ((cons fn-call &) term)
+         (formula (acl2::meta-extract-formula-w fn-call (w state)))
+         ((unless (pseudo-termp formula))
+          (prog2$
+           (er hard? 'expand-cp=>function-substitution "expand-cp: formula got by
        meta-extract is not a pseudo-termp.")
-         nil))
-       ((mv ok lhs rhs)
-        (case-match formula
-          (('equal lhs rhs)
-           (mv t lhs rhs))
-          (& (mv nil nil nil))))
-       ((unless (and ok (pseudo-termp lhs)))
-        (prog2$ (er hard? 'expand-cp=>function-substitution "expand-cp: formula got by
+           nil))
+         ((mv ok lhs rhs)
+          (case-match formula
+            (('equal lhs rhs)
+             (mv t lhs rhs))
+            (& (mv nil nil nil))))
+         ((unless (and ok (pseudo-termp lhs)))
+          (prog2$ (er hard? 'expand-cp=>function-substitution "expand-cp: formula got by
        meta-extract is not an equality.")
-                nil))
-       ((mv match-ok subst)
-        (acl2::simple-one-way-unify lhs term nil))
-       ((unless match-ok)
-        (prog2$
-         (er hard? 'expand-cp=>function-substitution "expand-cp:
+                  nil))
+         ((mv match-ok subst)
+          (acl2::simple-one-way-unify lhs term nil))
+         ((unless match-ok)
+          (prog2$
+           (er hard? 'expand-cp=>function-substitution "expand-cp:
        simple-one-way-unify failed.")
-         nil)))
-    `(equal ,term ,(acl2::substitute-into-term rhs subst))))
+           nil)))
+      `(equal ,term ,(acl2::substitute-into-term rhs subst))))
 
-(encapsulate()
-(local (in-theory (e/d (function-substitution) (w))))
+  (encapsulate()
+    (local (in-theory (e/d (function-substitution) (w))))
 
-(defthm function-substitution-correct
-  (implies (and (expev-meta-extract-global-facts)
-                (pseudo-termp term)
-                (alistp a)
-                (function-substitution term state))
-           (expev (function-substitution term state) a))
-  :hints (("Goal"
-           :in-theory (e/d ()
-                           (expev-meta-extract-formula))
-           :use ((:instance
-                  expev-meta-extract-formula
-                  (name (car term))
-                  (st state)
-                  (a (expev-alist
-                      (mv-nth 1
-                              (acl2::simple-one-way-unify
-                               (cadr (meta-extract-formula (car term) state))
-                               term nil))
-                      a))))
-           ))
-  )
-)
+    (defthm function-substitution-correct
+      (implies (and (expev-meta-extract-global-facts)
+                    (pseudo-termp term)
+                    (alistp a)
+                    (function-substitution term state))
+               (expev (function-substitution term state) a))
+      :hints (("Goal"
+               :in-theory (e/d ()
+                               (expev-meta-extract-formula))
+               :use ((:instance
+                      expev-meta-extract-formula
+                      (name (car term))
+                      (st state)
+                      (a (expev-alist
+                          (mv-nth 1
+                                  (acl2::simple-one-way-unify
+                                   (cadr (meta-extract-formula (car term) state))
+                                   term nil))
+                          a))))
+               ))
+      )
+    )
 
-(encapsulate ()
-  (local
-   (defthm type-of-assoc-equal-of-sym-nat-alistp
-     (implies (and (sym-nat-alistp x)
-                   (symbolp y)
-                   (assoc-equal y x))
-              (and (symbolp (car (assoc-equal y x)))
-                   (natp (cdr (assoc-equal y x))))))
-   )
+  (encapsulate ()
+    (local
+     (defthm type-of-assoc-equal-of-sym-nat-alistp
+       (implies (and (sym-nat-alistp x)
+                     (symbolp y)
+                     (assoc-equal y x))
+                (and (symbolp (car (assoc-equal y x)))
+                     (natp (cdr (assoc-equal y x))))))
+     )
 
-  (define fact-finder ((term pseudo-termp)
-                       (expand-args ex-args-p)
-                       state)
-    :guard (and (not (acl2::variablep term))
-                (not (acl2::fquotep term))
-                (symbolp (car term))
-                (not (assoc-equal term (ex-args->facts expand-args)))
-                (not (zp (ex-args->wrld-fn-len expand-args))))
-    :guard-hints (("Goal"
-                   :in-theory (e/d ()
-                                   (type-of-assoc-equal-of-sym-nat-alistp))
-                   :use ((:instance type-of-assoc-equal-of-sym-nat-alistp
-                                    (x (ex-args->fn-lvls expand-args))
-                                    (y (car term))))))
-    :returns (mv (new-term pseudo-termp)
-                 (new-args ex-args-p))
-    :short "Find the definition fact for @('term')"
-    :long "<p>Given a pseudo-termp @('term') that is not a @('variablep'), not
+    (define fact-finder ((term pseudo-termp)
+                         (expand-args ex-args-p)
+                         state)
+      :guard (and (not (acl2::variablep term))
+                  (not (acl2::fquotep term))
+                  (symbolp (car term))
+                  (not (assoc-equal term (ex-args->facts expand-args)))
+                  (not (zp (ex-args->wrld-fn-len expand-args))))
+      :guard-hints (("Goal"
+                     :in-theory (e/d ()
+                                     (type-of-assoc-equal-of-sym-nat-alistp))
+                     :use ((:instance type-of-assoc-equal-of-sym-nat-alistp
+                                      (x (ex-args->fn-lvls expand-args))
+                                      (y (car term))))))
+      :returns (mv (new-term pseudo-termp)
+                   (new-args ex-args-p))
+      :short "Find the definition fact for @('term')"
+      :long "<p>Given a pseudo-termp @('term') that is not a @('variablep'), not
 a @('fquotep'), nor a @('pseudo-lambdap'), and that it doesn't exist in the
 list of facts learnt @('(ex-args->facts expand-args)'), we want to find the
 definition fact of that term.</p>
 "
-    (b* ((term (pseudo-term-fix term))
-         (expand-args (ex-args-fix expand-args))
-         ((ex-args a) expand-args)
-         ((cons fn &) term)
-         ;; There are three cases:
-         ;; 1. fn is a basic function (including fty functions) -- fn-lvls stays
-         ;; the same, nothing is expanded, no fact generated
-         ;; For 2 and 3, if fn-lvls is already 0, then do nothing; if fn-lvls is
-         ;; not 0, expand.
-         ;; 2. fn exists in user-defined fn-lvls -- fn-lvls decrease by 1, fn is
-         ;; expanded, one fact generated
-         ;; 3. otherwise, fn will be expanded once -- fn-lvls decrease by 1, fn
-         ;; is expanded, one fact generated
-         (basic-function (member-equal fn *SMT-basics*))
-         (flex? (fncall-of-flextype fn a.fty-info))
-         (basic-fix (member-equal fn (strip-cdrs *SMT-fixers*)))
-         ((if (or basic-function flex? basic-fix))
-          (mv nil a))
-         (lvl (assoc-equal fn a.fn-lvls))
-         (user-defined (assoc-equal fn a.fn-lst))
-         ((if (and lvl (zp (cdr lvl)) user-defined)) (mv nil a))
-         ((if (and lvl (zp (cdr lvl)) (null user-defined)))
-          (prog2$ (er hard? 'expand-cp=>fact-finder "Possibly
+      (b* ((term (pseudo-term-fix term))
+           (expand-args (ex-args-fix expand-args))
+           ((ex-args a) expand-args)
+           ((cons fn &) term)
+           ;; There are three cases:
+           ;; 1. fn is a basic function (including fty functions) -- fn-lvls stays
+           ;; the same, nothing is expanded, no fact generated
+           ;; For 2 and 3, if fn-lvls is already 0, then do nothing; if fn-lvls is
+           ;; not 0, expand.
+           ;; 2. fn exists in user-defined fn-lvls -- fn-lvls decrease by 1, fn is
+           ;; expanded, one fact generated
+           ;; 3. otherwise, fn will be expanded once -- fn-lvls decrease by 1, fn
+           ;; is expanded, one fact generated
+           (basic-function (member-equal fn *SMT-basics*))
+           (flex? (fncall-of-flextype fn a.fty-info))
+           (basic-fix (member-equal fn (strip-cdrs *SMT-fixers*)))
+           ((if (or basic-function flex? basic-fix))
+            (mv nil a))
+           (lvl (assoc-equal fn a.fn-lvls))
+           (user-defined (assoc-equal fn a.fn-lst))
+           ((if (and lvl (zp (cdr lvl)) user-defined)) (mv nil a))
+           ((if (and lvl (zp (cdr lvl)) (null user-defined)))
+            (prog2$ (er hard? 'expand-cp=>fact-finder "Possibly
                        encountered recursive functions that are not
                        user-defined: ~q0" term)
-                  (mv nil a)))
-         (fact (function-substitution term state))
-         ((if (null fact)) (mv nil a))
-         ((if lvl)
-          (mv fact
-              (make-ex-args :fn-lvls (update-fn-lvls fn a.fn-lvls)
-                            :fn-lst a.fn-lst
-                            :facts (acons term fact a.facts)
-                            :fty-info a.fty-info
-                            :wrld-fn-len a.wrld-fn-len))))
-      ;; if not in fn-lvls
-      (mv fact
-          (make-ex-args :fn-lst a.fn-lst
-                        :fn-lvls (cons `(,fn . 0) a.fn-lvls)
-                        :facts (acons term fact a.facts)
-                        :fty-info a.fty-info
-                        :wrld-fn-len (1- a.wrld-fn-len))))
-    ///
-    (more-returns
-     (new-args
-      (implies
-       (and (pseudo-termp term)
-            (ex-args-p expand-args)
-            (symbolp (car term))
-            new-term
-            (assoc-equal (car term)
-                         (ex-args->fn-lvls expand-args)))
-       (and (< (sum-lvls (ex-args->fn-lvls new-args))
-               (sum-lvls (ex-args->fn-lvls expand-args)))
-            (equal (ex-args->wrld-fn-len new-args)
-                   (ex-args->wrld-fn-len expand-args))))
+                    (mv nil a)))
+           (fact (function-substitution term state))
+           ((if (null fact)) (mv nil a))
+           ((if lvl)
+            (mv fact
+                (make-ex-args :fn-lvls (update-fn-lvls fn a.fn-lvls)
+                              :fn-lst a.fn-lst
+                              :facts (acons term fact a.facts)
+                              :fty-info a.fty-info
+                              :wrld-fn-len a.wrld-fn-len))))
+        ;; if not in fn-lvls
+        (mv fact
+            (make-ex-args :fn-lst a.fn-lst
+                          :fn-lvls (cons `(,fn . 0) a.fn-lvls)
+                          :facts (acons term fact a.facts)
+                          :fty-info a.fty-info
+                          :wrld-fn-len (1- a.wrld-fn-len))))
+      ///
+      (more-returns
+       (new-args
+        (implies
+         (and (pseudo-termp term)
+              (ex-args-p expand-args)
+              (symbolp (car term))
+              new-term
+              (assoc-equal (car term)
+                           (ex-args->fn-lvls expand-args)))
+         (and (< (sum-lvls (ex-args->fn-lvls new-args))
+                 (sum-lvls (ex-args->fn-lvls expand-args)))
+              (equal (ex-args->wrld-fn-len new-args)
+                     (ex-args->wrld-fn-len expand-args))))
+        :hints (("Goal"
+                 :in-theory (e/d ()
+                                 (sum-lvls-decrease-after-update))
+                 :use ((:instance sum-lvls-decrease-after-update
+                                  (fn (car term))
+                                  (fn-lvls (ex-args->fn-lvls expand-args))))))
+        :name fact-finder-decrease-1)
+       (new-args
+        (implies
+         (and (pseudo-termp term)
+              (ex-args-p expand-args)
+              (symbolp (car term))
+              (not (zp (ex-args->wrld-fn-len expand-args)))
+              new-term
+              (not (assoc-equal (car term)
+                                (ex-args->fn-lvls expand-args))))
+         (< (ex-args->wrld-fn-len new-args)
+            (ex-args->wrld-fn-len expand-args)))
+        :name fact-finder-decrease-2)
+       (new-args
+        (implies (not new-term)
+                 (and (equal (ex-args->wrld-fn-len new-args)
+                             (ex-args->wrld-fn-len expand-args))
+                      (equal (sum-lvls (ex-args->fn-lvls new-args))
+                             (sum-lvls (ex-args->fn-lvls expand-args)))))
+        :name fact-finder-same-3)
+       )
+      )
+    )
+
+  (encapsulate ()
+    (local
+     (defthm acl2-count-of-last-of-consp-decrease
+       (implies (consp x)
+                (< (acl2-count (pseudo-term-fix (car (last x))))
+                   (acl2-count x)))
+       :hints (("Goal"
+                :in-theory (enable pseudo-term-fix)))
+       ))
+
+    (local
+     (defthm symbolp-of-fn-call-of-pseudo-termp
+       (implies (and (pseudo-termp x)
+                     (consp x)
+                     (not (acl2::fquotep x))
+                     (not (pseudo-lambdap (car x))))
+                (symbolp (car x)))
+       :hints (("Goal" :in-theory (enable pseudo-lambdap)))))
+
+    (defines transform
+      :well-founded-relation l<
+      :flag-local nil
+      :flag-defthm-macro defthm-transform
+      :verify-guards nil
+
+      (define transform-list ((term-lst pseudo-term-listp))
+        :returns (new-term-lst pseudo-term-listp)
+        :measure (acl2-count (pseudo-term-list-fix term-lst))
+        (b* ((term-lst (pseudo-term-list-fix term-lst))
+             ((unless (consp term-lst)) term-lst)
+             ((cons first rest) term-lst)
+             (first-term (transform first)))
+          (cons first-term
+                (transform-list rest))))
+
+      (define transform ((term pseudo-termp))
+        :returns (new-term pseudo-termp)
+        :measure (acl2-count (pseudo-term-fix term))
+        :hints (("Goal"
+                 :in-theory (e/d ()
+                                 (acl2-count-of-last-of-consp-decrease))
+                 :use ((:instance acl2-count-of-last-of-consp-decrease
+                                  (x (cdr (pseudo-term-fix term)))))))
+        (b* ((term (pseudo-term-fix term))
+             ;; If first term is a symbolp or is quoted, return the current facts
+             ((if (or (acl2::variablep term) (acl2::fquotep term))) term)
+             ;; The first term is now a function call:
+             ;; Cons the function call and function actuals out of term
+             ((cons fn-call fn-actuals) term)
+             ;; If fn-call is a pseudo-lambdap, transform the body
+             ((if (pseudo-lambdap fn-call))
+              (b* (((list 'lambda formal-lst body) fn-call)
+                   (transformed-body (transform body))
+                   (transformed-actuals (transform-list fn-actuals)))
+                (lambda-substitution `(lambda ,formal-lst
+                                        ,transformed-body)
+                                     transformed-actuals)))
+             ;; If fn-call is neither a lambda expression nor a function call
+             ((unless (mbt (symbolp fn-call))) nil)
+
+             ;; -----------------------------------------------------------
+             ;; Now the term is a function call
+             ((if (and (equal fn-call 'acl2::return-last)
+                       (equal (len fn-actuals) 3)))
+              (transform (car (last term)))))
+          (cons fn-call (transform-list fn-actuals))))
+      )
+
+    (local
+     (defthm tranform-list-maintain-length
+       (implies (pseudo-term-listp term-lst)
+                (equal (len (transform-list term-lst))
+                       (len term-lst)))
+       :hints (("Goal"
+                :expand (transform-list term-lst))))
+     )
+
+    (local
+     (defthm pseudo-lambdap-of-reconstruction
+       (implies (and (pseudo-termp term)
+                     (consp term)
+                     (not (equal 'quote (car term)))
+                     (pseudo-lambdap (car term)))
+                (pseudo-lambdap (list 'lambda
+                                      (cadr (car term))
+                                      (transform (caddr (car term))))))
+       :hints (("Goal"
+                :in-theory (enable pseudo-lambdap)))))
+
+    (local
+     (defthm pseudo-termp-of-car-of-last-of-return-last
+       (implies (and (pseudo-term-listp x)
+                     (consp x))
+                (pseudo-termp (car (last x))))
+       :hints (("Goal"
+                :in-theory (enable pseudo-term-listp last)))
+       ))
+
+    (verify-guards transform)
+
+    (defines induction-scheme
+      :well-founded-relation l<
+      :flag-local nil
+      :verify-guards nil
+
+      (define induction-scheme-list ((term-lst pseudo-term-listp)
+                                     (al))
+        (declare (irrelevant al))
+        :measure (acl2-count (pseudo-term-list-fix term-lst))
+        (b* ((term-lst (pseudo-term-list-fix term-lst))
+             ((unless (consp term-lst)) term-lst)
+             ((cons first rest) term-lst))
+          (cons (induction-scheme first al)
+                (induction-scheme-list rest al))))
+
+      (define induction-scheme ((term pseudo-termp)
+                                (al))
+        (declare (irrelevant al))
+        :measure (acl2-count (pseudo-term-fix term))
+        :hints (("Goal"
+                 :in-theory (e/d ()
+                                 (acl2-count-of-last-of-consp-decrease))
+                 :use ((:instance acl2-count-of-last-of-consp-decrease
+                                  (x (cdr (pseudo-term-fix term)))))))
+        (b* ((term (pseudo-term-fix term))
+             ;; If first term is a symbolp or is quoted, return the current facts
+             ((if (or (acl2::variablep term) (acl2::fquotep term))) term)
+             ;; The first term is now a function call:
+             ;; Cons the function call and function actuals out of term
+             ((cons fn-call fn-actuals) term)
+             ;; If fn-call is a pseudo-lambdap, transform the body
+             ((if (pseudo-lambdap fn-call))
+              (b* (((list 'lambda formal-lst body) fn-call)
+                   ;; (transformed-body (transform body))
+                   ;; (transformed-actuals (transform-list fn-actuals)))
+                   )
+                (lambda-substitution
+                 (induction-scheme body
+                                   (pairlis$ formal-lst
+                                             (expev-lst fn-actuals al)))
+                 (induction-scheme-list fn-actuals al))))
+             ;; If fn-call is neither a lambda expression nor a function call
+             ((unless (mbt (symbolp fn-call))) nil)
+
+             ;; -----------------------------------------------------------
+             ;; Now the term is a function call
+             ((if (and (equal fn-call 'acl2::return-last)
+                       (equal (len fn-actuals) 3)))
+              (induction-scheme (car (last term)) al)))
+          (induction-scheme-list fn-actuals al)))
+      )
+
+    (local
+     (defthm induction-scheme-list-maintain-length
+       (implies (pseudo-term-listp term-lst)
+                (equal (len (induction-scheme-list term-lst al))
+                       (len term-lst)))
+       :hints (("Goal"
+                :expand ((induction-scheme-list term-lst al)
+                         (induction-scheme-list nil al)))))
+     )
+
+    (local
+     (defthm cdr-of-transform-list
+       (implies (pseudo-term-listp x)
+                (equal (transform-list (cdr x))
+                       (cdr (transform-list x))))
+       :hints (("Goal"
+                :expand (transform-list x)))
+       ))
+
+    (local
+     (defthm crock1
+       (implies (equal (len x) 1)
+                (equal (car (last x))
+                       (car x)))
+       :hints (("Goal"
+                :in-theory (enable last len)))))
+
+    (defthm-induction-scheme-flag
+      (defthm transform-pseudo-termp
+        (implies (and (expev-meta-extract-global-facts)
+                      (pseudo-termp term)
+                      (alistp a))
+                 (equal (expev (transform term) a)
+                        (expev term a)))
+        :hints ('(:expand ((transform term))
+                          :in-theory (e/d (expev-of-fncall-args)
+                                          (lambda-substitution-correct))
+                          :use ((:instance lambda-substitution-correct
+                                           (fn-call (list 'lambda
+                                                          (cadr (car term))
+                                                          (transform (caddr (car term)))))
+                                           (fn-actuals (transform-list (cdr term)))
+                                           (a a)))))
+        :flag induction-scheme)
+      (defthm transform-pseudo-term-listp
+        (implies (and (expev-meta-extract-global-facts)
+                      (pseudo-term-listp term-lst)
+                      (alistp a))
+                 (equal (expev-lst (transform-list term-lst) a)
+                        (expev-lst term-lst a)))
+        :hints ('(:expand ((transform-list term-lst)
+                           (transform-list nil))))
+        :flag induction-scheme-list)
+      :hints(("Goal" :induct (induction-scheme-flag flag term-lst term a))))
+
+    (defthm transform-implies-function-substitution
+      (implies (and (pseudo-termp term)
+                    (transform (function-substitution term state)))
+               (function-substitution term state))
+      :hints (("Goal"
+               :in-theory (e/d (transform)
+                               ()))))
+
+    (defthm transform-function-substitution-correct
+      (implies (and (expev-meta-extract-global-facts)
+                    (pseudo-termp term)
+                    (alistp a)
+                    (transform (function-substitution term state)))
+               (expev (transform (function-substitution term state)) a))
+      :hints (("Goal"
+               :in-theory (e/d (transform) ()))))
+
+    (defines expand
+      :well-founded-relation l<
+      :flag-local nil
+      :verify-guards nil
+      :flag-defthm-macro defthm-expand
+
+      (define expand-list ((term-lst pseudo-term-listp)
+                           (expand-args ex-args-p)
+                           state)
+        :returns (fact-alst fact-alistp)
+        :measure (list (ex-args->wrld-fn-len expand-args)
+                       (sum-lvls (ex-args->fn-lvls expand-args))
+                       (acl2-count (pseudo-term-list-fix term-lst)))
+        (b* ((term-lst (pseudo-term-list-fix term-lst))
+             (expand-args (ex-args-fix expand-args))
+             ((ex-args a) expand-args)
+             ((unless (consp term-lst)) a.facts)
+             ((cons first rest) term-lst)
+             (facts-first (expand first a state)))
+          (expand-list rest (change-ex-args a :facts facts-first) state)))
+
+      (define expand ((term pseudo-termp)
+                      (expand-args ex-args-p)
+                      state)
+        :returns (fact-alst fact-alistp)
+        :measure (list (ex-args->wrld-fn-len expand-args)
+                       (sum-lvls (ex-args->fn-lvls expand-args))
+                       (acl2-count (pseudo-term-fix term)))
+        :hints (("Goal"
+                 :in-theory (e/d ()
+                                 (fact-finder-decrease-1
+                                  fact-finder-decrease-2
+                                  fact-finder-same-3))
+                 :use ((:instance fact-finder-decrease-1
+                                  (term (pseudo-term-fix term))
+                                  (expand-args (ex-args-fix expand-args)))
+                       (:instance fact-finder-decrease-2
+                                  (term (pseudo-term-fix term))
+                                  (expand-args (ex-args-fix expand-args)))
+                       (:instance fact-finder-same-3
+                                  (term (pseudo-term-fix term))
+                                  (expand-args (ex-args-fix expand-args)))
+                       (:instance acl2-count-of-last-of-consp-decrease
+                                  (x (cdr (pseudo-term-fix term))))
+                       )))
+        (b* ((term (pseudo-term-fix term))
+             (expand-args (ex-args-fix expand-args))
+             ((ex-args a) expand-args)
+             ((if (zp a.wrld-fn-len)) a.facts)
+             ;; If first term is a symbolp or is quoted, return the current facts
+             ((if (or (acl2::variablep term) (acl2::fquotep term))) a.facts)
+             ;; The first term is now a function call:
+             ;; Cons the function call and function actuals out of term
+             ((cons fn-call fn-actuals) term)
+             ;; If fn-call is a pseudo-lambdap, substitute unbounded variables in the
+             ;; lambda and recurse to expand the substituted term.
+             ;; To ensure termination, wrld-fn-len needs to decrease, this means
+             ;; wrld-fn-len should include term size so that it's large enough.
+             ((if (pseudo-lambdap fn-call))
+              (expand (lambda-substitution fn-call fn-actuals)
+                      (change-ex-args a :wrld-fn-len (1- a.wrld-fn-len))
+                      state))
+             ;; If fn-call is neither a lambda expression nor a function call
+             ((unless (mbt (symbolp fn-call))) nil)
+
+             ;; -----------------------------------------------------------
+             ;; Now the term is a function call we first test if term already
+             ;; exists in facts alist.
+             (exists? (assoc-equal term a.facts))
+             ;; I can skip the whole subtree because if such a term already exists in
+             ;; facts, then it's subterms, subsubterms ... must also exist in the
+             ;; facts. This is because we are doing a depth first travesal.
+             ((if exists?) a.facts)
+             ((mv new-term new-args) (fact-finder term a state))
+             ;; new-term being nil meaning there's no fact to prove
+             ((unless new-term)
+              (expand-list fn-actuals new-args state)))
+          (expand new-term new-args state)))
+      )
+
+    (verify-guards expand)
+    )
+
+  (define initialize-fn-lvls ((fn-lst func-alistp))
+    :returns (fn-lvls sym-nat-alistp)
+    :measure (len fn-lst)
+    :hints (("Goal" :in-theory (enable func-alist-fix)))
+    (b* ((fn-lst (func-alist-fix fn-lst))
+         ((unless (consp fn-lst)) nil)
+         ((cons first rest) fn-lst)
+         ((func f) (cdr first)))
+      (cons (cons f.name f.expansion-depth) (initialize-fn-lvls rest))))
+
+  (define compose-goal ((cl pseudo-term-listp)
+                        (to-be-learnt pseudo-term-listp)
+                        state)
+    :returns (new-goal pseudo-term-listp)
+    :measure (len (pseudo-term-list-fix to-be-learnt))
+    (b* ((cl (pseudo-term-list-fix cl))
+         (to-be-learnt (pseudo-term-list-fix to-be-learnt))
+         ((unless (consp to-be-learnt)) cl)
+         ((cons first-fact rest-facts) to-be-learnt)
+         ((unless (and (not (acl2::variablep first-fact))
+                       (not (acl2::fquotep first-fact))
+                       (symbolp (car first-fact))))
+          cl)
+         (learnt-fact (transform (function-substitution first-fact state)))
+         ((if (null learnt-fact)) cl))
+      `((not ,learnt-fact)
+        ,@(compose-goal cl rest-facts state))))
+
+  (encapsulate ()
+    (local (in-theory (e/d (compose-goal) ())))
+
+    (local
+     (defthm expev-of-disjoin
+       (iff (expev (disjoin clause) a)
+            (acl2::or-list (expev-lst clause a)))
+       :hints(("Goal" :in-theory (enable acl2::or-list len)
+               :induct (len clause)))))
+
+    (defthm compose-goal-correct
+      (implies (and (expev-meta-extract-global-facts)
+                    (pseudo-term-listp clause)
+                    (alistp a)
+                    (expev (disjoin
+                            (compose-goal clause to-be-learnt state))
+                           a))
+               (expev (disjoin clause) a))
       :hints (("Goal"
                :in-theory (e/d ()
-                               (sum-lvls-decrease-after-update))
-               :use ((:instance sum-lvls-decrease-after-update
-                                (fn (car term))
-                                (fn-lvls (ex-args->fn-lvls expand-args))))))
-      :name fact-finder-decrease-1)
-     (new-args
-      (implies
-       (and (pseudo-termp term)
-            (ex-args-p expand-args)
-            (symbolp (car term))
-            (not (zp (ex-args->wrld-fn-len expand-args)))
-            new-term
-            (not (assoc-equal (car term)
-                              (ex-args->fn-lvls expand-args))))
-       (< (ex-args->wrld-fn-len new-args)
-          (ex-args->wrld-fn-len expand-args)))
-      :name fact-finder-decrease-2)
-     (new-args
-      (implies (not new-term)
-               (and (equal (ex-args->wrld-fn-len new-args)
-                           (ex-args->wrld-fn-len expand-args))
-                    (equal (sum-lvls (ex-args->fn-lvls new-args))
-                           (sum-lvls (ex-args->fn-lvls expand-args)))))
-      :name fact-finder-same-3)
-     )
+                               (expev-of-disjoin
+                                transform-pseudo-termp))
+               :use
+               ((:instance function-substitution-correct
+                           (term (car (pseudo-term-list-fix to-be-learnt)))
+                           (a a)
+                           (state state))
+                (:instance transform-pseudo-termp
+                           (term (function-substitution
+                                  (car (pseudo-term-list-fix to-be-learnt))
+                                  state))
+                           (a a))
+                ))))
+
+    (defthm compose-transformed-goal-correct
+      (implies (and (expev-meta-extract-global-facts)
+                    (pseudo-term-listp clause)
+                    (alistp a)
+                    (expev
+                     (disjoin
+                      (compose-goal (transform-list clause)
+                                    to-be-learnt state))
+                     a))
+               (expev (disjoin clause) a)))
     )
-  )
 
-(encapsulate ()
-(local
- (defthm acl2-count-of-last-of-consp-decrease
-   (implies (consp x)
-            (< (acl2-count (pseudo-term-fix (car (last x))))
-               (acl2-count x)))
-   :hints (("Goal"
-            :in-theory (enable pseudo-term-fix)))
-   ))
+  (encapsulate ()
+    (local
+     (defthm pseudo-term-listp-of-strip-cars-of-fact-alistp
+       (implies (fact-alistp x)
+                (pseudo-term-listp (strip-cars x)))))
 
-(local
- (defthm symbolp-of-fn-call-of-pseudo-termp
-   (implies (and (pseudo-termp x)
-                 (consp x)
-                 (not (acl2::fquotep x))
-                 (not (pseudo-lambdap (car x))))
-            (symbolp (car x)))
-   :hints (("Goal" :in-theory (enable pseudo-lambdap)))))
+    (define expand-cp-helper ((cl pseudo-term-listp)
+                              (smtlink-hint t)
+                              state)
+      :returns (subgoal-lst pseudo-term-list-listp)
+      (b* (((unless (pseudo-term-listp cl)) nil)
+           ((unless (smtlink-hint-p smtlink-hint))
+            (list cl))
+           ;; generate all fty related stuff
+           (flextypes-table (table-alist 'fty::flextypes-table (w state)))
+           ((unless (alistp flextypes-table)) (list cl))
+           (h1 (generate-fty-info-alist smtlink-hint flextypes-table))
+           (h2 (generate-fty-types-top h1 flextypes-table))
+           ((smtlink-hint h) h2)
+           ;; Make an alist version of fn-lst
+           (fn-lst (make-alist-fn-lst h.functions))
+           (fn-lvls (initialize-fn-lvls fn-lst))
+           (wrld-fn-len h.wrld-fn-len)
+           (transformed-cl (transform-list cl))
+           ;; Do function expansion
+           (facts nil)
+           (to-be-learnt
+            (with-fast-alists (facts fn-lvls fn-lst)
+              (expand (disjoin transformed-cl)
+                      (make-ex-args
+                       :fn-lvls fn-lvls
+                       :fn-lst fn-lst
+                       :facts facts
+                       :fty-info h.fty-info
+                       :wrld-fn-len wrld-fn-len)
+                      state)))
+           (expanded-goal (compose-goal transformed-cl (strip-cars to-be-learnt) state))
+           (next-cp (cdr (assoc-equal 'expand *SMT-architecture*)))
+           ((if (null next-cp)) (list cl))
+           (the-hint
+            `(:clause-processor (,next-cp clause ',h)))
+           (hinted-goal `((hint-please ',the-hint) ,@expanded-goal)))
+        (list hinted-goal)))
+    )
 
-(defines transform
-  :well-founded-relation l<
-  :flag-local nil
-  :flag-defthm-macro defthm-transform
-  :verify-guards nil
+  (define expand-cp ((cl pseudo-term-listp)
+                     (hints t)
+                     state)
+    (b* ((expanded-clause (expand-cp-helper cl hints state)))
+      (value expanded-clause)))
 
-  (define transform-list ((term-lst pseudo-term-listp))
-    :returns (new-term-lst pseudo-term-listp)
-    :measure (acl2-count (pseudo-term-list-fix term-lst))
-    (b* ((term-lst (pseudo-term-list-fix term-lst))
-         ((unless (consp term-lst)) term-lst)
-         ((cons first rest) term-lst)
-         (first-term (transform first)))
-      (cons first-term
-            (transform-list rest))))
+  (local (in-theory (enable expand-cp expand-cp-helper)))
 
-  (define transform ((term pseudo-termp))
-    :returns (new-term pseudo-termp)
-    :measure (acl2-count (pseudo-term-fix term))
-    :hints (("Goal"
-             :in-theory (e/d ()
-                             (acl2-count-of-last-of-consp-decrease))
-             :use ((:instance acl2-count-of-last-of-consp-decrease
-                              (x (cdr (pseudo-term-fix term)))))))
-    (b* ((term (pseudo-term-fix term))
-         ;; If first term is a symbolp or is quoted, return the current facts
-         ((if (or (acl2::variablep term) (acl2::fquotep term))) term)
-         ;; The first term is now a function call:
-         ;; Cons the function call and function actuals out of term
-         ((cons fn-call fn-actuals) term)
-         ;; If fn-call is a pseudo-lambdap, transform the body
-         ((if (pseudo-lambdap fn-call))
-          (b* (((list 'lambda formal-lst body) fn-call)
-               (transformed-body (transform body))
-               (transformed-actuals (transform-list fn-actuals))
-               ((unless (mbt (equal (len formal-lst)
-                                    (len transformed-actuals))))
-                nil))
-            (cons `(lambda ,formal-lst ,transformed-body)
-                  transformed-actuals)))
-         ;; If fn-call is neither a lambda expression nor a function call
-         ((unless (mbt (symbolp fn-call))) nil)
-
-         ;; -----------------------------------------------------------
-         ;; Now the term is a function call
-         ((if (and (equal fn-call 'acl2::return-last)
-                   (equal (len fn-actuals) 3)))
-          (transform (car (last term)))))
-      (cons fn-call (transform-list fn-actuals))))
-  )
-
-(local
-(defthm tranform-list-maintain-length
-  (implies (pseudo-term-listp term-lst)
-           (equal (len (transform-list term-lst))
-                  (len term-lst)))
-  :hints (("Goal"
-           :expand (transform-list term-lst))))
-)
-
-(local
- (defthm pseudo-termp-of-car-of-last-of-return-last
-   (implies (and (pseudo-term-listp x)
-                 (consp x))
-            (pseudo-termp (car (last x))))
-   :hints (("Goal"
-            :in-theory (enable pseudo-term-listp last)))
-   ))
-
-(verify-guards transform)
-
-(defines induction-scheme
-  :well-founded-relation l<
-  :flag-local nil
-  :verify-guards nil
-
-  (define induction-scheme-list ((term-lst pseudo-term-listp)
-                                 (al))
-    (declare (irrelevant al))
-    :measure (acl2-count (pseudo-term-list-fix term-lst))
-    (b* ((term-lst (pseudo-term-list-fix term-lst))
-         ((unless (consp term-lst)) term-lst)
-         ((cons first rest) term-lst))
-      (cons (induction-scheme first al)
-            (induction-scheme-list rest al))))
-
-  (define induction-scheme ((term pseudo-termp)
-                            (al))
-    (declare (irrelevant al))
-    :measure (acl2-count (pseudo-term-fix term))
-    :hints (("Goal"
-             :in-theory (e/d ()
-                             (acl2-count-of-last-of-consp-decrease))
-             :use ((:instance acl2-count-of-last-of-consp-decrease
-                              (x (cdr (pseudo-term-fix term)))))))
-    (b* ((term (pseudo-term-fix term))
-         ;; If first term is a symbolp or is quoted, return the current facts
-         ((if (or (acl2::variablep term) (acl2::fquotep term))) term)
-         ;; The first term is now a function call:
-         ;; Cons the function call and function actuals out of term
-         ((cons fn-call fn-actuals) term)
-         ;; If fn-call is a pseudo-lambdap, transform the body
-         ((if (pseudo-lambdap fn-call))
-          (b* (((list 'lambda formal-lst body) fn-call)
-               ;; (transformed-body (transform body))
-               ;; (transformed-actuals (transform-list fn-actuals))
-               ((unless (mbt (equal (len formal-lst)
-                                    (len fn-actuals))))
-                nil))
-            (cons (induction-scheme body
-                                    (pairlis$ formal-lst
-                                              (expev-lst fn-actuals al)))
-                  (induction-scheme-list fn-actuals al))))
-         ;; If fn-call is neither a lambda expression nor a function call
-         ((unless (mbt (symbolp fn-call))) nil)
-
-         ;; -----------------------------------------------------------
-         ;; Now the term is a function call
-         ((if (and (equal fn-call 'acl2::return-last)
-                   (equal (len fn-actuals) 3)))
-          (induction-scheme (car (last term)) al)))
-      (induction-scheme-list fn-actuals al)))
-  )
-
-(local
- (defthm induction-scheme-list-maintain-length
-   (implies (pseudo-term-listp term-lst)
-            (equal (len (induction-scheme-list term-lst al))
-                   (len term-lst)))
-   :hints (("Goal"
-            :expand ((induction-scheme-list term-lst al)
-                     (induction-scheme-list nil al)))))
- )
-
-(local
- (defthm cdr-of-transform-list
-   (implies (pseudo-term-listp x)
-            (equal (transform-list (cdr x))
-                   (cdr (transform-list x))))
-   :hints (("Goal"
-            :expand (transform-list x)))
-   ))
-
-(local
- (defthm crock1
-   (implies (equal (len x) 1)
-            (equal (car (last x))
-                   (car x)))
-   :hints (("Goal"
-            :in-theory (enable last len)))))
-
-(defthm-induction-scheme-flag
-  (defthm transform-pseudo-termp
+  (defthm correctness-of-expand-cp
     (implies (and (expev-meta-extract-global-facts)
-                  (pseudo-termp term))
-             (equal (expev (transform term) a)
-                    (expev term a)))
-    :hints ('(:expand ((transform term))
-                      :in-theory (enable expev-of-fncall-args)))
-    :flag induction-scheme)
-  (defthm transform-pseudo-term-listp
-    (implies (and (expev-meta-extract-global-facts)
-                  (pseudo-term-listp term-lst))
-             (equal (expev-lst (transform-list term-lst) a)
-                    (expev-lst term-lst a)))
-    :hints ('(:expand ((transform-list term-lst)
-                       (transform-list nil))))
-    :flag induction-scheme-list)
-  :hints(("Goal" :induct (induction-scheme-flag flag term-lst term a))))
-
-(defines expand
-  :well-founded-relation l<
-  :flag-local nil
-  :verify-guards nil
-  :flag-defthm-macro defthm-expand
-
-  (define expand-list ((term-lst pseudo-term-listp)
-                       (expand-args ex-args-p)
-                       state)
-    :returns (fact-alst fact-alistp)
-    :measure (list (ex-args->wrld-fn-len expand-args)
-                   (sum-lvls (ex-args->fn-lvls expand-args))
-                   (acl2-count (pseudo-term-list-fix term-lst)))
-    (b* ((term-lst (pseudo-term-list-fix term-lst))
-         (expand-args (ex-args-fix expand-args))
-         ((ex-args a) expand-args)
-         ((unless (consp term-lst)) a.facts)
-         ((cons first rest) term-lst)
-         (facts-first (expand first a state)))
-      (expand-list rest (change-ex-args a :facts facts-first) state)))
-
-  (define expand ((term pseudo-termp)
-                  (expand-args ex-args-p)
-                  state)
-    :returns (fact-alst fact-alistp)
-    :measure (list (ex-args->wrld-fn-len expand-args)
-                   (sum-lvls (ex-args->fn-lvls expand-args))
-                   (acl2-count (pseudo-term-fix term)))
-    :hints (("Goal"
-             :in-theory (e/d ()
-                             (fact-finder-decrease-1
-                              fact-finder-decrease-2
-                              fact-finder-same-3))
-             :use ((:instance fact-finder-decrease-1
-                              (term (pseudo-term-fix term))
-                              (expand-args (ex-args-fix expand-args)))
-                   (:instance fact-finder-decrease-2
-                              (term (pseudo-term-fix term))
-                              (expand-args (ex-args-fix expand-args)))
-                   (:instance fact-finder-same-3
-                              (term (pseudo-term-fix term))
-                              (expand-args (ex-args-fix expand-args)))
-                   (:instance acl2-count-of-last-of-consp-decrease
-                              (x (cdr (pseudo-term-fix term))))
-                   )))
-    (b* ((term (pseudo-term-fix term))
-         (expand-args (ex-args-fix expand-args))
-         ((ex-args a) expand-args)
-         ((if (zp a.wrld-fn-len)) a.facts)
-         ;; If first term is a symbolp or is quoted, return the current facts
-         ((if (or (acl2::variablep term) (acl2::fquotep term))) a.facts)
-         ;; The first term is now a function call:
-         ;; Cons the function call and function actuals out of term
-         ((cons fn-call fn-actuals) term)
-         ;; If fn-call is a pseudo-lambdap, substitute unbounded variables in the
-         ;; lambda and recurse to expand the substituted term.
-         ;; To ensure termination, wrld-fn-len needs to decrease, this means
-         ;; wrld-fn-len should include term size so that it's large enough.
-         ((if (pseudo-lambdap fn-call))
-          (expand (lambda-substitution fn-call fn-actuals)
-                  (change-ex-args a :wrld-fn-len (1- a.wrld-fn-len))
-                  state))
-         ;; If fn-call is neither a lambda expression nor a function call
-         ((unless (mbt (symbolp fn-call))) nil)
-
-         ;; -----------------------------------------------------------
-         ;; Now the term is a function call we first test if term already
-         ;; exists in facts alist.
-         (exists? (assoc-equal term a.facts))
-         ;; I can skip the whole subtree because if such a term already exists in
-         ;; facts, then it's subterms, subsubterms ... must also exist in the
-         ;; facts. This is because we are doing a depth first travesal.
-         ((if exists?) a.facts)
-         ((mv new-term new-args) (fact-finder term a state))
-         ;; new-term being nil meaning there's no fact to prove
-         ((unless new-term)
-          (expand-list fn-actuals new-args state)))
-      (expand new-term new-args state)))
+                  (pseudo-term-listp clause)
+                  (alistp a)
+                  (expev
+                   (conjoin-clauses
+                    (acl2::clauses-result
+                     (expand-cp clause hints state)))
+                   a))
+             (expev (disjoin clause) a))
+    :rule-classes :clause-processor)
   )
-
-(verify-guards expand)
-)
-
-(define initialize-fn-lvls ((fn-lst func-alistp))
-  :returns (fn-lvls sym-nat-alistp)
-  :measure (len fn-lst)
-  :hints (("Goal" :in-theory (enable func-alist-fix)))
-  (b* ((fn-lst (func-alist-fix fn-lst))
-       ((unless (consp fn-lst)) nil)
-       ((cons first rest) fn-lst)
-       ((func f) (cdr first)))
-    (cons (cons f.name f.expansion-depth) (initialize-fn-lvls rest))))
-
-(define compose-goal ((cl pseudo-term-listp)
-                      (to-be-learnt pseudo-term-listp)
-                      state)
-  :returns (new-goal pseudo-term-listp)
-  :measure (len (pseudo-term-list-fix to-be-learnt))
-  (b* ((cl (pseudo-term-list-fix cl))
-       (to-be-learnt (pseudo-term-list-fix to-be-learnt))
-       ((unless (consp to-be-learnt)) cl)
-       ((cons first-fact rest-facts) to-be-learnt)
-       ((unless (and (not (acl2::variablep first-fact))
-                     (not (acl2::fquotep first-fact))
-                     (symbolp (car first-fact))))
-        cl)
-       (learnt-fact (function-substitution first-fact state))
-       ((if (null learnt-fact)) cl))
-    `((not ,learnt-fact)
-      ,@(compose-goal cl rest-facts state))))
-
-(encapsulate ()
-(local (in-theory (e/d (compose-goal) ())))
-
-(local
- (defthm expev-of-disjoin
-   (iff (expev (disjoin clause) a)
-        (acl2::or-list (expev-lst clause a)))
-   :hints(("Goal" :in-theory (enable acl2::or-list len)
-           :induct (len clause)))))
-
-(defthm compose-goal-correct
-  (implies (and (expev-meta-extract-global-facts)
-                (pseudo-term-listp clause)
-                (alistp a)
-                (expev (disjoin
-                        (compose-goal clause to-be-learnt state))
-                       a))
-           (expev (disjoin clause) a))
-  :hints (("Goal"
-           :in-theory (disable expev-of-disjoin)
-           :expand (compose-goal clause to-be-learnt state)
-           :use
-           ((:instance function-substitution-correct
-                       (term (car (pseudo-term-list-fix to-be-learnt)))
-                       (a a)
-                       (state state)))
-           ))
-  )
-
-(defthm compose-transformed-goal-correct
-  (implies (and (expev-meta-extract-global-facts)
-                (pseudo-term-listp clause)
-                (alistp a)
-                (expev
-                 (disjoin
-                  (compose-goal (transform-list clause) to-be-learnt state))
-                 a))
-           (expev (disjoin clause) a)))
-)
-
-(encapsulate ()
-  (local
-   (defthm pseudo-term-listp-of-strip-cars-of-fact-alistp
-     (implies (fact-alistp x)
-              (pseudo-term-listp (strip-cars x)))))
-
-(define expand-cp-helper ((cl pseudo-term-listp)
-                          (smtlink-hint t)
-                          state)
-  :returns (subgoal-lst pseudo-term-list-listp)
-  (b* (((unless (pseudo-term-listp cl)) nil)
-       ((unless (smtlink-hint-p smtlink-hint))
-        (list cl))
-       ;; generate all fty related stuff
-       (flextypes-table (table-alist 'fty::flextypes-table (w state)))
-       ((unless (alistp flextypes-table)) (list cl))
-       (h1 (generate-fty-info-alist smtlink-hint flextypes-table))
-       (h2 (generate-fty-types-top h1 flextypes-table))
-       ((smtlink-hint h) h2)
-       ;; Make an alist version of fn-lst
-       (fn-lst (make-alist-fn-lst h.functions))
-       (fn-lvls (initialize-fn-lvls fn-lst))
-       (wrld-fn-len h.wrld-fn-len)
-       (transformed-cl (transform-list cl))
-       ;; Do function expansion
-       (facts nil)
-       (to-be-learnt
-        (with-fast-alists (facts fn-lvls fn-lst)
-          (expand (disjoin transformed-cl)
-                  (make-ex-args
-                   :fn-lvls fn-lvls
-                   :fn-lst fn-lst
-                   :facts facts
-                   :fty-info h.fty-info
-                   :wrld-fn-len wrld-fn-len)
-                  state)))
-       (expanded-goal (compose-goal transformed-cl (strip-cars to-be-learnt) state))
-       (next-cp (cdr (assoc-equal 'expand *SMT-architecture*)))
-       ((if (null next-cp)) (list cl))
-       (the-hint
-        `(:clause-processor (,next-cp clause ',h)))
-       (hinted-goal `((hint-please ',the-hint) ,@expanded-goal)))
-    (list hinted-goal)))
-)
-
-(define expand-cp ((cl pseudo-term-listp)
-                   (hints t)
-                   state)
-  (b* ((expanded-clause (expand-cp-helper cl hints state)))
-    (value expanded-clause)))
-
-(local (in-theory (enable expand-cp expand-cp-helper)))
-
-(defthm correctness-of-expand-cp
-  (implies (and (expev-meta-extract-global-facts)
-                (pseudo-term-listp clause)
-                (alistp a)
-                (expev
-                 (conjoin-clauses
-                  (acl2::clauses-result
-                   (expand-cp clause hints state)))
-                 a))
-           (expev (disjoin clause) a))
-  :rule-classes :clause-processor)
-)
