books/projects/smtlink/verified/uninterpreted-fn-cp.lisp
@@ -76,401 +76,405 @@
       type-thm-w/o-lambda))
 
 
-    ;; BOZO: Should be able to do functional-instantiation of
-    ;; lambda-substitution-correct, but I got lost at the symbols from package acl2
-    ;; and current package
-    (local (defthm unev-alist-of-pairlis$
-             (equal (unev-alist (pairlis$ x y) a)
-                    (pairlis$ x (unev-lst y a)))))
+  ;; BOZO: Should be able to do functional-instantiation of
+  ;; lambda-substitution-correct, but I got lost at the symbols from package acl2
+  ;; and current package
+  (local (defthm unev-alist-of-pairlis$
+           (equal (unev-alist (pairlis$ x y) a)
+                  (pairlis$ x (unev-lst y a)))))
 
-    (defthm lambda-substitution-correct-uninterpreted
-      (implies (and (unev-meta-extract-global-facts)
-                    (alistp a)
-                    (pseudo-lambdap fn-call)
-                    (pseudo-term-listp fn-actuals))
-               (equal
-                (unev (lambda-substitution fn-call fn-actuals) a)
-                (unev (cons fn-call fn-actuals) a)))
-      :hints (("Goal"
-               :in-theory (enable lambda-substitution))))
+  (defthm lambda-substitution-correct-uninterpreted
+    (implies (and (unev-meta-extract-global-facts)
+                  (alistp a)
+                  (pseudo-lambdap fn-call)
+                  (pseudo-term-listp fn-actuals))
+             (equal
+              (unev (lambda-substitution fn-call fn-actuals) a)
+              (unev (cons fn-call fn-actuals) a)))
+    :hints (("Goal"
+             :in-theory (enable lambda-substitution))))
 
-    (defthm type-thm-remove-lambda-correct
-      (implies (and (unev-meta-extract-global-facts)
-                    (alistp a))
-               (or (null (type-thm-remove-lambda func state))
-                   (unev (type-thm-remove-lambda func state) a)))
-      :hints (("Goal"
-               :do-not-induct t
-               :in-theory (e/d (type-thm-remove-lambda
-                                unev-of-fncall-args)
-                               (pseudo-term-listp
-                                pseudo-termp
-                                car-cdr-elim
-                                w
-                                lambda-substitution-correct-uninterpreted))
-               :use ((:instance
-                      lambda-substitution-correct-uninterpreted
-                      (a a)
-                      (fn-call
-                       (car (meta-extract-formula (car (func->meta-extract-thms func))
-                                                  state)))
-                      (fn-actuals
-                       (cdr (meta-extract-formula (car (func->meta-extract-thms func))
-                                                  state)))
-                      ))
-               )))
+  (defthm type-thm-remove-lambda-correct
+    (implies (and (unev-meta-extract-global-facts)
+                  (alistp a))
+             (or (null (type-thm-remove-lambda func state))
+                 (unev (type-thm-remove-lambda func state) a)))
+    :hints (("Goal"
+             :do-not-induct t
+             :in-theory (e/d (type-thm-remove-lambda
+                              unev-of-fncall-args)
+                             (pseudo-term-listp
+                              pseudo-termp
+                              car-cdr-elim
+                              w
+                              lambda-substitution-correct-uninterpreted))
+             :use ((:instance
+                    lambda-substitution-correct-uninterpreted
+                    (a a)
+                    (fn-call
+                     (car (meta-extract-formula (car (func->meta-extract-thms func))
+                                                state)))
+                    (fn-actuals
+                     (cdr (meta-extract-formula (car (func->meta-extract-thms func))
+                                                state)))
+                    ))
+             )))
 
-    (define uninterpreted-substitution ((term pseudo-termp)
-                                        (type-thm pseudo-termp))
-      :returns (new-term pseudo-termp
-                         :hints (("Goal"
-                                  :in-theory (enable pseudo-termp
-                                                     pseudo-term-fix
-                                                     pairlis$))))
-      (b* ((term (pseudo-term-fix term))
-           (type-thm (pseudo-term-fix type-thm))
-           (vars (reverse (acl2::simple-term-vars type-thm)))
-           (- (cw "vars: ~q0" vars))
-           (- (cw "vars term: ~q0" term))
-           ((unless (and (consp term)
-                         (acl2::pseudo-term-substp (pairlis$ vars (cdr term)))))
-            (prog2$ (er hard? 'uninterpreted-fn-cp=>uninterpreted-substitution
-                        "acl2::simple-term-vars failed with ~p0
+  (local
+   (defthm alistp-of-pairlis$
+     (alistp (pairlis$ keys vals)))
+   )
+
+  (define uninterpreted-substitution ((term pseudo-termp)
+                                      (type-thm pseudo-termp))
+    :returns (new-term pseudo-termp
+                       :hints (("Goal"
+                                :in-theory (enable pseudo-termp
+                                                   pseudo-term-fix
+                                                   pairlis$))))
+    (b* ((term (pseudo-term-fix term))
+         (type-thm (pseudo-term-fix type-thm))
+         (vars (reverse (acl2::simple-term-vars type-thm)))
+         (- (cw "vars: ~q0" vars))
+         (- (cw "vars term: ~q0" term))
+         ((unless (and (consp term)
+                       (acl2::pseudo-term-substp (pairlis$ vars (cdr term)))))
+          (prog2$ (er hard? 'uninterpreted-fn-cp=>uninterpreted-substitution
+                      "acl2::simple-term-vars failed with ~p0
                                     and ~p1" type-thm term)
-                    nil)))
-        (acl2::substitute-into-term type-thm (pairlis$ vars (cdr term)))))
+                  nil)))
+      (acl2::substitute-into-term type-thm (pairlis$ vars (cdr term)))))
 
-    (define type-thm-full ((term pseudo-termp)
-                           (func func-p)
-                           state)
-      :returns (new-term pseudo-termp)
-      (b* ((term (pseudo-term-fix term))
-           (type-thm-w/o-lambda (type-thm-remove-lambda func state))
-           ((unless type-thm-w/o-lambda)
-            (prog2$ (er hard? 'uninterpreted-fn-cp=>type-thm-full
-                        "Something is wrong with type-thm-remove-lambda.")
-                    nil))
-           (type-thm (uninterpreted-substitution term type-thm-w/o-lambda))
-           ((unless type-thm)
-            (prog2$ (er hard? 'uninterpreted-fn-cp=>type-thm-full
-                        "Something is wrong with uninterpreted-substitution.")
-                    nil)))
-        type-thm))
+  (define type-thm-full ((term pseudo-termp)
+                         (func func-p)
+                         state)
+    :returns (new-term pseudo-termp)
+    (b* ((term (pseudo-term-fix term))
+         (type-thm-w/o-lambda (type-thm-remove-lambda func state))
+         ((unless type-thm-w/o-lambda)
+          (prog2$ (er hard? 'uninterpreted-fn-cp=>type-thm-full
+                      "Something is wrong with type-thm-remove-lambda.")
+                  nil))
+         (type-thm (uninterpreted-substitution term type-thm-w/o-lambda))
+         ((unless type-thm)
+          (prog2$ (er hard? 'uninterpreted-fn-cp=>type-thm-full
+                      "Something is wrong with uninterpreted-substitution.")
+                  nil)))
+      type-thm))
 
-    (local (defthm alistp-of-unev-alist (alistp (unev-alist x a))))
+  (local (defthm alistp-of-unev-alist (alistp (unev-alist x a))))
 
-    (defthm type-thm-full-correct
-      (implies (and (unev-meta-extract-global-facts)
-                    (alistp a)
-                    (pseudo-termp term))
-               (or (null (type-thm-full term func state))
-                   (unev (type-thm-full term func state) a)))
-      :hints (("Goal"
-               :do-not-induct t
-               :in-theory (e/d (type-thm-full
-                                uninterpreted-substitution)
-                               (type-thm-remove-lambda-correct))
-               :use ((:instance type-thm-remove-lambda-correct
-                                (func func)
-                                (a (pairlis$
-                                    (reverse (acl2::simple-term-vars
-                                              (type-thm-remove-lambda func state)))
-                                    (unev-lst (cdr term) a)))))
-               )))
+  (defthm type-thm-full-correct
+    (implies (and (unev-meta-extract-global-facts)
+                  (alistp a)
+                  (pseudo-termp term))
+             (or (null (type-thm-full term func state))
+                 (unev (type-thm-full term func state) a)))
+    :hints (("Goal"
+             :do-not-induct t
+             :in-theory (e/d (type-thm-full
+                              uninterpreted-substitution)
+                             (type-thm-remove-lambda-correct))
+             :use ((:instance type-thm-remove-lambda-correct
+                              (func func)
+                              (a (pairlis$
+                                  (reverse (acl2::simple-term-vars
+                                            (type-thm-remove-lambda func state)))
+                                  (unev-lst (cdr term) a)))))
+             )))
 
 
-    (define fix-thm-meta-extract ((func func-p)
-                                  state)
-      :returns (new-term pseudo-termp)
-      (b* ((func (func-fix func))
-           (thms (func->meta-extract-thms func))
-           ((mv ok type-fix-when-type)
-            (case-match thms
-              ((& type-fix-when-type)
-               (mv t type-fix-when-type))
-              (& (mv nil nil))))
-           ((unless ok)
-            (er hard? 'uninterpreted-fn-cp=>fix-thm-meta-extract "Smtlink need two theorems
+  (define fix-thm-meta-extract ((func func-p)
+                                state)
+    :returns (new-term pseudo-termp)
+    (b* ((func (func-fix func))
+         (thms (func->meta-extract-thms func))
+         ((mv ok type-fix-when-type)
+          (case-match thms
+            ((& type-fix-when-type)
+             (mv t type-fix-when-type))
+            (& (mv nil nil))))
+         ((unless ok)
+          (er hard? 'uninterpreted-fn-cp=>fix-thm-meta-extract "Smtlink need two theorems
  to justify the proof of return types of uninterpreted functions. Expected
  [type-of-f] and [type-fix-when-type], but got: ~q0" thms))
-           (- (cw "type-fix-when-type: ~q0" type-fix-when-type))
-           (fix-thm (acl2::meta-extract-formula-w type-fix-when-type (w
-                                                                      state)))
-           (- (cw "fix-thm1: ~q0" fix-thm))
-           ((unless (and (pseudo-termp fix-thm) (not (equal fix-thm ''t))))
-            (er hard? 'uninterpreted-fn-cp=>fix-thm-meta-extract "Type theorem
+         (- (cw "type-fix-when-type: ~q0" type-fix-when-type))
+         (fix-thm (acl2::meta-extract-formula-w type-fix-when-type (w
+                                                                    state)))
+         (- (cw "fix-thm1: ~q0" fix-thm))
+         ((unless (and (pseudo-termp fix-thm) (not (equal fix-thm ''t))))
+          (er hard? 'uninterpreted-fn-cp=>fix-thm-meta-extract "Type theorem
                               type-of-f is not of the expected shape: ~q0"
-                fix-thm)))
-        fix-thm))
+              fix-thm)))
+      fix-thm))
 
-    (defthm fix-thm-meta-extract-correct
-      (implies (and (unev-meta-extract-global-facts)
-                    (alistp a))
-               (or (null (fix-thm-meta-extract func state))
-                   (unev (fix-thm-meta-extract func state) a)))
-      :hints (("Goal"
-               :do-not-induct t
-               :in-theory (e/d (fix-thm-meta-extract
-                                unev-of-fncall-args)
-                               (pseudo-term-listp
-                                pseudo-termp
-                                car-cdr-elim
-                                w))
-               )))
+  (defthm fix-thm-meta-extract-correct
+    (implies (and (unev-meta-extract-global-facts)
+                  (alistp a))
+             (or (null (fix-thm-meta-extract func state))
+                 (unev (fix-thm-meta-extract func state) a)))
+    :hints (("Goal"
+             :do-not-induct t
+             :in-theory (e/d (fix-thm-meta-extract
+                              unev-of-fncall-args)
+                             (pseudo-term-listp
+                              pseudo-termp
+                              car-cdr-elim
+                              w))
+             )))
 
-    (define fix-thm-full ((term pseudo-termp)
-                          (func func-p)
-                          state)
-      :returns (new-term pseudo-termp)
-      :guard-debug t
-      (b* ((term (pseudo-term-fix term))
-           (fix-thm (fix-thm-meta-extract func state))
-           ((unless fix-thm)
-            (er hard? 'uninterpreted-fn-cp=>fix-thm-full
-                "Something is wrong with fix-thm-meta-extract."))
-           (vars (reverse (acl2::simple-term-vars fix-thm)))
-           (- (cw "fix-thm: ~q0" fix-thm))
-           ((unless (and (consp vars) (null (cdr vars))))
-            (er hard? 'uninterpreted-fn-cp=>fix-thm-full
-                "Free vars from fix-thm: ~q0" vars)))
-        (acl2::substitute-into-term fix-thm (pairlis$ vars (list term)))))
-
-    (defthm fix-thm-full-correct
-      (implies (and (unev-meta-extract-global-facts)
-                    (alistp a)
-                    (pseudo-termp term))
-               (or (null (fix-thm-full term func state))
-                   (unev (fix-thm-full term func state) a)))
-      :hints (("Goal"
-               :do-not-induct t
-               :in-theory (e/d (fix-thm-full)
-                               (fix-thm-meta-extract-correct))
-               :use ((:instance fix-thm-meta-extract-correct
-                                (func func)
-                                (a (list
-                                    (cons (car (reverse
-                                                (acl2::simple-term-vars
-                                                 (fix-thm-meta-extract func state))))
-                                          (unev term a))))))
-               )))
-
-    (define find-fixer ((term pseudo-termp)
+  (define fix-thm-full ((term pseudo-termp)
                         (func func-p)
                         state)
-      :returns (fixer pseudo-termp)
-      (b* ((type-thm (type-thm-full term func state))
-           ((unless type-thm)
-            (er hard? 'uninterpreted-fn-cp=>find-fixer
-                "Something is wrong with type-thm-full."))
-           (fix-thm (fix-thm-full term func state))
-           ((unless fix-thm)
-            (er hard? 'uninterpreted-fn-cp=>find-fixer
-                "Something is wrong with fix-thm-full."))
-           (- (cw "fix-thm: ~q0" fix-thm))
-           (- (cw "type-thm: ~q0" type-thm))
-           (- (cw "term: ~q0" term))
-           ((mv ok fixed type-thm term)
-            (case-match fix-thm
-              (('implies type-thm
-                         ('equal fixed term))
-               (mv t fixed type-thm term))
-              (& (mv nil nil nil nil))))
-           (- (cw "fixed: ~p0, type-thm: ~p1, term: ~p2~%" fixed type-thm term))
-           ((unless (and ok (pseudo-termp fixed)))
-            (er hard? 'uninterpreted-fn-cp=>find-fixer
-                "Fixer wrong: ~q0" fixed)))
-        fixed))
+    :returns (new-term pseudo-termp)
+    :guard-debug t
+    (b* ((term (pseudo-term-fix term))
+         (fix-thm (fix-thm-meta-extract func state))
+         ((unless fix-thm)
+          (er hard? 'uninterpreted-fn-cp=>fix-thm-full
+              "Something is wrong with fix-thm-meta-extract."))
+         (vars (reverse (acl2::simple-term-vars fix-thm)))
+         (- (cw "fix-thm: ~q0" fix-thm))
+         ((unless (and (consp vars) (null (cdr vars))))
+          (er hard? 'uninterpreted-fn-cp=>fix-thm-full
+              "Free vars from fix-thm: ~q0" vars)))
+      (acl2::substitute-into-term fix-thm (pairlis$ vars (list term)))))
 
-    (defthm find-fixer-correct
-      (implies (and (unev-meta-extract-global-facts)
-                    (alistp a)
-                    (pseudo-termp term))
-               (or (null (find-fixer term func state))
-                   (equal (unev (find-fixer term func state) a)
-                          (unev term a))))
-      :hints (("Goal"
-               :in-theory (e/d (find-fixer
-                                unev-of-fncall-args)
-                               (pseudo-term-listp
-                                pseudo-termp
-                                car-cdr-elim
-                                w
-                                fix-thm-full-correct
-                                type-thm-full-correct))
-               :use ((:instance fix-thm-full-correct
-                                (a a)
-                                (term term)
-                                (func func))
-                     (:instance type-thm-full-correct
-                                (a a)
-                                (term term)
-                                (func func)))
-               )))
+  (defthm fix-thm-full-correct
+    (implies (and (unev-meta-extract-global-facts)
+                  (alistp a)
+                  (pseudo-termp term))
+             (or (null (fix-thm-full term func state))
+                 (unev (fix-thm-full term func state) a)))
+    :hints (("Goal"
+             :do-not-induct t
+             :in-theory (e/d (fix-thm-full)
+                             (fix-thm-meta-extract-correct))
+             :use ((:instance fix-thm-meta-extract-correct
+                              (func func)
+                              (a (list
+                                  (cons (car (reverse
+                                              (acl2::simple-term-vars
+                                               (fix-thm-meta-extract func state))))
+                                        (unev term a))))))
+             )))
 
-    (defines uninterpreted
-      :well-founded-relation l<
-      :flag-local nil
-      :flag-defthm-macro defthm-uninterpreted
-      :verify-guards nil
+  (define find-fixer ((term pseudo-termp)
+                      (func func-p)
+                      state)
+    :returns (fixer pseudo-termp)
+    (b* ((type-thm (type-thm-full term func state))
+         ((unless type-thm)
+          (er hard? 'uninterpreted-fn-cp=>find-fixer
+              "Something is wrong with type-thm-full."))
+         (fix-thm (fix-thm-full term func state))
+         ((unless fix-thm)
+          (er hard? 'uninterpreted-fn-cp=>find-fixer
+              "Something is wrong with fix-thm-full."))
+         (- (cw "fix-thm: ~q0" fix-thm))
+         (- (cw "type-thm: ~q0" type-thm))
+         (- (cw "term: ~q0" term))
+         ((mv ok fixed)
+          (case-match fix-thm
+            (('implies !type-thm
+                       ('equal fixed !term))
+             (mv t fixed))
+            (& (mv nil nil))))
+         ((unless (and ok (pseudo-termp fixed)))
+          (er hard? 'uninterpreted-fn-cp=>find-fixer
+              "Fixer wrong: ~q0" fixed)))
+      fixed))
 
-      (define uninterpreted-list ((term-lst pseudo-term-listp)
-                                  (fn-lst func-alistp)
-                                  (fty-info fty-info-alist-p)
-                                  state)
-        :returns (new-term-lst pseudo-term-listp)
-        :measure (acl2-count (pseudo-term-list-fix term-lst))
-        :hints (("Goal" :in-theory (enable pseudo-term-list-fix
-                                           pseudo-term-fix)))
-        (b* ((term-lst (pseudo-term-list-fix term-lst))
-             ((unless (consp term-lst)) term-lst)
-             ((cons first rest) term-lst)
-             (first-term (uninterpreted first fn-lst fty-info state)))
-          (cons first-term
-                (uninterpreted-list rest fn-lst fty-info state))))
+  (defthm find-fixer-correct
+    (implies (and (unev-meta-extract-global-facts)
+                  (alistp a)
+                  (pseudo-termp term))
+             (or (null (find-fixer term func state))
+                 (equal (unev (find-fixer term func state) a)
+                        (unev term a))))
+    :hints (("Goal"
+             :in-theory (e/d (find-fixer
+                              unev-of-fncall-args)
+                             (pseudo-term-listp
+                              pseudo-termp
+                              car-cdr-elim
+                              w
+                              fix-thm-full-correct
+                              type-thm-full-correct))
+             :use ((:instance fix-thm-full-correct
+                              (a a)
+                              (term term)
+                              (func func))
+                   (:instance type-thm-full-correct
+                              (a a)
+                              (term term)
+                              (func func)))
+             )))
 
-      (define uninterpreted ((term pseudo-termp)
-                             (fn-lst func-alistp)
-                             (fty-info fty-info-alist-p)
-                             state)
-        :returns (new-term pseudo-termp)
-        :measure (acl2-count (pseudo-term-fix term))
-        (b* ((term (pseudo-term-fix term))
-             ;; (fn-lst (func-alist-fix fn-lst))
-             ;; If first term is a symbolp or is quoted, return the current facts
-             ((if (or (acl2::variablep term) (acl2::fquotep term))) term)
-             ;; The first term is now a function call:
-             ;; Cons the function call and function actuals out of term
-             ((cons fn-call fn-actuals) term)
-             ;; If fn-call is a pseudo-lambdap, transform the body
-             ((if (pseudo-lambdap fn-call))
-              (prog2$ (er hard? 'uninterpreted-fn-cp=>uninterpreted "There still
+  (defines uninterpreted
+    :well-founded-relation l<
+    :flag-local nil
+    :flag-defthm-macro defthm-uninterpreted
+    :verify-guards nil
+
+    (define uninterpreted-list ((term-lst pseudo-term-listp)
+                                (fn-lst func-alistp)
+                                (fty-info fty-info-alist-p)
+                                state)
+      :returns (new-term-lst pseudo-term-listp)
+      :measure (acl2-count (pseudo-term-list-fix term-lst))
+      :hints (("Goal" :in-theory (enable pseudo-term-list-fix
+                                         pseudo-term-fix)))
+      (b* ((term-lst (pseudo-term-list-fix term-lst))
+           ((unless (consp term-lst)) term-lst)
+           ((cons first rest) term-lst)
+           (first-term (uninterpreted first fn-lst fty-info state)))
+        (cons first-term
+              (uninterpreted-list rest fn-lst fty-info state))))
+
+    (define uninterpreted ((term pseudo-termp)
+                           (fn-lst func-alistp)
+                           (fty-info fty-info-alist-p)
+                           state)
+      :returns (new-term pseudo-termp)
+      :measure (acl2-count (pseudo-term-fix term))
+      (b* ((term (pseudo-term-fix term))
+           ;; (fn-lst (func-alist-fix fn-lst))
+           ;; If first term is a symbolp or is quoted, return the current facts
+           ((if (or (acl2::variablep term) (acl2::fquotep term))) term)
+           ;; The first term is now a function call:
+           ;; Cons the function call and function actuals out of term
+           ((cons fn-call fn-actuals) term)
+           ;; If fn-call is a pseudo-lambdap, transform the body
+           ((if (pseudo-lambdap fn-call))
+            (prog2$ (er hard? 'uninterpreted-fn-cp=>uninterpreted "There still
                            exists lambda in the term. Very strange.~%~q0~%" term)
-                      term))
-             ;; If fn-call is neither a lambda expression nor a function call
-             ((unless (mbt (symbolp fn-call))) nil)
-             ((if (equal fn-call 'type-hyp)) term)
+                    term))
+           ;; If fn-call is neither a lambda expression nor a function call
+           ((unless (mbt (symbolp fn-call))) nil)
+           ((if (equal fn-call 'type-hyp)) term)
 
-             ;; -----------------------------------------------------------
-             ;; Now the term is a function call
-             (basic-function (member-equal fn-call *SMT-basics*))
-             (flex? (fncall-of-flextype fn-call fty-info))
-             ((if (or basic-function flex?))
-              (cons fn-call
-                    (uninterpreted-list fn-actuals fn-lst fty-info state)))
-             ;; fn-call is not a basic function nor a flex function
-             (user-defined (assoc-equal fn-call fn-lst))
-             ((unless user-defined)
-              (prog2$ (er hard? 'uninterpreted-fn-cp=>uninterpreted "User hasn't
+           ;; -----------------------------------------------------------
+           ;; Now the term is a function call
+           (basic-function (member-equal fn-call *SMT-basics*))
+           (flex? (fncall-of-flextype fn-call fty-info))
+           ((if (or basic-function flex?))
+            (cons fn-call
+                  (uninterpreted-list fn-actuals fn-lst fty-info state)))
+           ;; fn-call is not a basic function nor a flex function
+           (user-defined (assoc-equal fn-call fn-lst))
+           ((unless user-defined)
+            (prog2$ (er hard? 'uninterpreted-fn-cp=>uninterpreted "User hasn't
 defined the uninterpreted function: ~q0" fn-call)
-                      term))
-             (fixed (find-fixer term (cdr user-defined) state))
-             ((mv ok fixer)
-              (case-match fixed
-                ((fixer (!fn-call . !fn-actuals))
-                 (mv t fixer))
-                (& (mv nil nil))))
-             ((unless (and ok (symbolp fixer)
-                           (not (equal fixer 'quote))))
-              (prog2$ (er hard? 'uninterpreted-fn-cp=>uninterpreted "Fixer wrong: ~q0" fixer)
-                      term)))
-          (list fixer
-                (cons fn-call (uninterpreted-list fn-actuals fn-lst
-                                                  fty-info state)))))
-      )
-
-    (encapsulate ()
-      (local
-       (defthm symbolp-of-car-of-pseudo-termp
-         (implies (and (consp term)
-                       (not (pseudo-lambdap (car term)))
-                       (pseudo-termp term))
-                  (symbolp (car term)))
-         :hints (("Goal" :in-theory (enable pseudo-lambdap pseudo-termp))))
-       )
-
-      (local
-       (defthm func-p-of-cdr-of-assoc-equal-of-func-alistp
-         (implies (and (func-alistp fn-lst)
-                       (assoc-equal (car term) fn-lst))
-                  (and (consp (assoc-equal (car term) fn-lst))
-                       (func-p (cdr (assoc-equal (car term) fn-lst)))))))
-
-      (verify-guards uninterpreted)
-
-      (defthm-uninterpreted
-        (defthm uninterpreted-term
-          (implies (and (unev-meta-extract-global-facts)
-                        (alistp a)
-                        (pseudo-termp term))
-                   (equal (unev
-                           (uninterpreted term fn-lst fty-info state) a)
-                          (unev term a)))
-          :hints ('(:expand ((uninterpreted term fn-lst fty-info state))
-                            :in-theory (e/d (unev-of-fncall-args)
-                                            (find-fixer-correct
-                                             member-equal
-                                             pseudo-term-listp
-                                             pseudo-termp
-                                             acl2::member-of-cons))
-                            :use ((:instance find-fixer-correct
-                                             (term term)
-                                             (a a)
-                                             (func (cdr (assoc-equal (car term) fn-lst)))))))
-          :flag uninterpreted)
-        (defthm uninterpreted-term-lst
-          (implies (and (unev-meta-extract-global-facts)
-                        (alistp a)
-                        (pseudo-term-listp term-lst))
-                   (equal (unev-lst
-                           (uninterpreted-list term-lst fn-lst fty-info state)
-                           a)
-                          (unev-lst term-lst a)))
-          :hints ('(:expand ((uninterpreted-list term-lst fn-lst fty-info state)
-                             (uninterpreted-list nil fn-lst fty-info state))))
-          :flag uninterpreted-list))
-      )
-
-    (define uninterpreted-fn ((cl pseudo-term-listp)
-                              (smtlink-hint t)
-                              state)
-      :returns (new-term pseudo-term-list-listp)
-      (b* (((unless (pseudo-term-listp cl)) nil)
-           (- (cw "cl: ~q0" cl))
-           ((unless (smtlink-hint-p smtlink-hint)) (list cl))
-           ;; generate all fty related stuff
-           (flextypes-table (table-alist 'fty::flextypes-table (w state)))
-           ((unless (alistp flextypes-table)) (list cl))
-           (h1 (generate-fty-info-alist smtlink-hint flextypes-table))
-           (h2 (generate-fty-types-top h1 flextypes-table))
-           ((smtlink-hint h) h2)
-           (fn-lst (make-alist-fn-lst h.functions))
-           (new-term (uninterpreted (disjoin cl) fn-lst h.fty-info state))
-           (next-cp (if h.custom-p
-                        (cdr (assoc-equal 'uninterpreted-custom
-                                          *SMT-architecture*))
-                      (cdr (assoc-equal 'uninterpreted *SMT-architecture*))))
-           ((if (null next-cp)) (list cl))
-           (the-hint
-            `(:clause-processor (,next-cp clause ',h state)))
-           (hinted-goal `((hint-please ',the-hint) ,new-term)))
-        (list hinted-goal)))
-
-    (define uninterpreted-fn-cp ((cl pseudo-term-listp)
-                                 (hints t)
-                                 state)
-      (b* ((fixed-clause (uninterpreted-fn cl hints state)))
-        (value fixed-clause)))
-
-    (local (in-theory (enable uninterpreted-fn-cp uninterpreted-fn)))
-
-    (defthm uninterpreted-fn-correct
-      (implies (and (unev-meta-extract-global-facts)
-                    (pseudo-term-listp clause)
-                    (alistp a)
-                    (unev (conjoin-clauses
-                           (acl2::clauses-result
-                            (uninterpreted-fn-cp clause hints state)))
-                          a))
-               (unev (disjoin clause) a))
-      :rule-classes :clause-processor)
+                    term))
+           (fixed (find-fixer term (cdr user-defined) state))
+           ((mv ok fixer)
+            (case-match fixed
+              ((fixer (!fn-call . !fn-actuals))
+               (mv t fixer))
+              (& (mv nil nil))))
+           ((unless (and ok (symbolp fixer)
+                         (not (equal fixer 'quote))))
+            (prog2$ (er hard? 'uninterpreted-fn-cp=>uninterpreted "Fixer wrong: ~q0" fixer)
+                    term)))
+        (list fixer
+              (cons fn-call (uninterpreted-list fn-actuals fn-lst
+                                                fty-info state)))))
     )
+
+  (encapsulate ()
+    (local
+     (defthm symbolp-of-car-of-pseudo-termp
+       (implies (and (consp term)
+                     (not (pseudo-lambdap (car term)))
+                     (pseudo-termp term))
+                (symbolp (car term)))
+       :hints (("Goal" :in-theory (enable pseudo-lambdap pseudo-termp))))
+     )
+
+    (local
+     (defthm func-p-of-cdr-of-assoc-equal-of-func-alistp
+       (implies (and (func-alistp fn-lst)
+                     (assoc-equal (car term) fn-lst))
+                (and (consp (assoc-equal (car term) fn-lst))
+                     (func-p (cdr (assoc-equal (car term) fn-lst)))))))
+
+    (verify-guards uninterpreted)
+
+    (defthm-uninterpreted
+      (defthm uninterpreted-term
+        (implies (and (unev-meta-extract-global-facts)
+                      (alistp a)
+                      (pseudo-termp term))
+                 (equal (unev
+                         (uninterpreted term fn-lst fty-info state) a)
+                        (unev term a)))
+        :hints ('(:expand ((uninterpreted term fn-lst fty-info state))
+                          :in-theory (e/d (unev-of-fncall-args)
+                                          (find-fixer-correct
+                                           member-equal
+                                           pseudo-term-listp
+                                           pseudo-termp
+                                           acl2::member-of-cons))
+                          :use ((:instance find-fixer-correct
+                                           (term term)
+                                           (a a)
+                                           (func (cdr (assoc-equal (car term) fn-lst)))))))
+        :flag uninterpreted)
+      (defthm uninterpreted-term-lst
+        (implies (and (unev-meta-extract-global-facts)
+                      (alistp a)
+                      (pseudo-term-listp term-lst))
+                 (equal (unev-lst
+                         (uninterpreted-list term-lst fn-lst fty-info state)
+                         a)
+                        (unev-lst term-lst a)))
+        :hints ('(:expand ((uninterpreted-list term-lst fn-lst fty-info state)
+                           (uninterpreted-list nil fn-lst fty-info state))))
+        :flag uninterpreted-list))
+    )
+
+  (define uninterpreted-fn ((cl pseudo-term-listp)
+                            (smtlink-hint t)
+                            state)
+    :returns (new-term pseudo-term-list-listp)
+    (b* (((unless (pseudo-term-listp cl)) nil)
+         (- (cw "cl: ~q0" cl))
+         ((unless (smtlink-hint-p smtlink-hint)) (list cl))
+         ;; generate all fty related stuff
+         (flextypes-table (table-alist 'fty::flextypes-table (w state)))
+         ((unless (alistp flextypes-table)) (list cl))
+         (h1 (generate-fty-info-alist smtlink-hint flextypes-table))
+         (h2 (generate-fty-types-top h1 flextypes-table))
+         ((smtlink-hint h) h2)
+         (fn-lst (make-alist-fn-lst h.functions))
+         (new-term (uninterpreted (disjoin cl) fn-lst h.fty-info state))
+         (next-cp (if h.custom-p
+                      (cdr (assoc-equal 'uninterpreted-custom
+                                        *SMT-architecture*))
+                    (cdr (assoc-equal 'uninterpreted *SMT-architecture*))))
+         ((if (null next-cp)) (list cl))
+         (the-hint
+          `(:clause-processor (,next-cp clause ',h state)))
+         (hinted-goal `((hint-please ',the-hint) ,new-term)))
+      (list hinted-goal)))
+
+  (define uninterpreted-fn-cp ((cl pseudo-term-listp)
+                               (hints t)
+                               state)
+    (b* ((fixed-clause (uninterpreted-fn cl hints state)))
+      (value fixed-clause)))
+
+  (local (in-theory (enable uninterpreted-fn-cp uninterpreted-fn)))
+
+  (defthm uninterpreted-fn-correct
+    (implies (and (unev-meta-extract-global-facts)
+                  (pseudo-term-listp clause)
+                  (alistp a)
+                  (unev (conjoin-clauses
+                         (acl2::clauses-result
+                          (uninterpreted-fn-cp clause hints state)))
+                        a))
+             (unev (disjoin clause) a))
+    :rule-classes :clause-processor)
+  )
